SystemFD/Metatheory/Inversion.lean
@@ -4,31 +4,41 @@ import SystemFD.Ctx
 import SystemFD.Metatheory.Weaken
 import SystemFD.Metatheory.Uniqueness
 import SystemFD.Metatheory.FrameWf
+import SystemFD.Metatheory.Classification
 
 theorem inversion_apply_spine :
   Γ ⊢ t.apply_spine sp : A ->
-  ∃ B, Γ ⊢ t : B
+  ∃ B, SpineType B A ∧ Γ ⊢ t : B
 := by
 intro j; induction sp generalizing Γ t A <;> simp at *
-case _ => exists A
+case _ => exists A; apply And.intro SpineType.refl j
 case _ hd tl ih =>
   cases hd; case _ v a =>
   cases v <;> simp at *
   case _ =>
     replace ih := ih j
     cases ih; case _ B ih =>
-    cases ih; case _ j1 j2 j3 =>
-    apply Exists.intro _; apply j1
+    cases ih; case _ h1 h2 =>
+    cases h2; case _ C D j1 j2 j3 =>
+      subst j3; apply Exists.intro (C -t> D)
+      apply And.intro; apply SpineType.arrow j2 h1
+      apply j1
   case _ =>
     replace ih := ih j
     cases ih; case _ B ih =>
-    cases ih; case _ j1 j2 j3 =>
-    apply Exists.intro _; apply j1
+    cases ih; case _ h1 h2 =>
+    cases h2; case _ C D j1 j2 j3 =>
+      subst j3; apply Exists.intro (∀[C] D)
+      apply And.intro; apply SpineType.all j2 h1
+      apply j1
   case _ =>
     replace ih := ih j
     cases ih; case _ B ih =>
-    cases ih; case _ j =>
-    apply Exists.intro _; apply j
+    cases ih; case _ j1 j2 =>
+    cases j2; case _ C j2 j3 =>
+      apply Exists.intro (C -k> B)
+      apply And.intro; apply SpineType.arrowk j1
+      apply j3
 
 theorem apply_spine_uniform :
   Γ ⊢ a : A ->
@@ -47,6 +57,7 @@ case _ hd tl ih =>
   case _ =>
     have lem := inversion_apply_spine j3
     cases lem; case _ D lem =>
+    cases lem; case _ lem =>
     cases lem; case _ U V q1 q2 q3 =>
       have lem1 := uniqueness_of_types j1 q1; subst lem1
       have lem2 : Γ ⊢ (a `@ t) : (V β[t]) := by
@@ -57,6 +68,7 @@ case _ hd tl ih =>
   case _ =>
     have lem := inversion_apply_spine j3
     cases lem; case _ D lem =>
+    cases lem; case _ lem =>
     cases lem; case _ U V q1 q2 q3 =>
       have lem1 := uniqueness_of_types j1 q1; subst lem1
       have lem2 : Γ ⊢ (a `@t t) : (V β[t]) := by
@@ -67,6 +79,7 @@ case _ hd tl ih =>
   case _ =>
     have lem := inversion_apply_spine j3
     cases lem; case _ D lem =>
+    cases lem; case _ lem =>
     cases lem; case _ U q1 q2 =>
       have lem1 := uniqueness_of_types j1 q2; subst lem1
       have lem2 : Γ ⊢ (a `@k t) : D := by
@@ -167,6 +180,160 @@ case _ j1 j2 =>
   subst h3; cases j2
   case _ j2 =>
     unfold ValidHeadVariable at j2; simp at j2
+
+theorem spine_type_is_not_kind :
+  SpineType A T ->
+  Γ ⊢ T : ★ ->
+  Γ ⊢ A : .kind ->
+  False
+:= by
+intro h1 h2 h3
+induction h1
+case _ =>
+  have lem := uniqueness_of_types h2 h3
+  injection lem
+case _ => cases h3
+case _ => cases h3
+case _ j ih =>
+  cases h3; case _ h3 =>
+    apply ih h2 h3
+
+theorem valid_ctor_not_equality :
+  ¬ (ValidCtor Γ (A ~ B))
+:= by
+intro h
+generalize Tdef : (A ~ B) = T at *
+induction h generalizing A B
+case _ j =>
+  unfold ValidHeadVariable at j; subst Tdef
+  simp at *
+case _ j ih => injection Tdef
+case _ => injection Tdef
+
+theorem spine_type_is_not_valid_ctor :
+  T = (C ~ D) ->
+  SpineType A T ->
+  ValidCtor Γ A ->
+  False
+:= by
+intro e h1 h2
+induction h1 generalizing C D Γ
+case _ =>
+  subst e; apply valid_ctor_not_equality h2
+case _ Γ a A B T j1 j2 ih =>
+  cases h2
+  case _ h =>
+    unfold ValidHeadVariable at h; simp at *
+  case _ h =>
+    apply @ih C D Γ e; apply valid_ctor_subst _ _ h
+    case _ =>
+      intro n y h1
+      cases n <;> simp at *
+      case _ n => subst h1; rw [Frame.apply_compose]; simp
+    case _ =>
+      intro n h1
+      cases n <;> simp at *
+      case _ =>
+        unfold Frame.apply at h1; simp at h1
+        unfold Frame.is_stable at h1; simp at h1
+case _ Γ a A B T j1 j2 ih =>
+  cases h2
+  case _ h =>
+    unfold ValidHeadVariable at h; simp at *
+  case _ h =>
+    apply @ih C D Γ e; apply valid_ctor_subst _ _ h
+    case _ =>
+      intro n y h1
+      cases n <;> simp at *
+      case _ n => subst h1; rw [Frame.apply_compose]; simp
+    case _ =>
+      intro n h1
+      cases n <;> simp at *
+      case _ =>
+        unfold Frame.apply at h1; simp at h1
+        unfold Frame.is_stable at h1; simp at h1
+case _ B T A j ih =>
+  cases h2; case _ h =>
+    unfold ValidHeadVariable at h; simp at *
+
+theorem valid_insttype_not_equality :
+  ¬ (ValidInstType Γ (A ~ B))
+:= by
+intro h
+generalize Tdef : (A ~ B) = T at *
+induction h generalizing A B
+case _ j =>
+  unfold ValidHeadVariable at j; subst Tdef
+  simp at *
+case _ j ih => injection Tdef
+case _ => injection Tdef
+
+theorem spine_type_is_not_valid_insttype :
+  T = (C ~ D) ->
+  SpineType A T ->
+  ValidInstType Γ A ->
+  False
+:= by
+intro e h1 h2
+induction h1 generalizing C D Γ
+case _ =>
+  subst e; apply valid_insttype_not_equality h2
+case _ Γ a A B T j1 j2 ih =>
+  cases h2
+  case _ h =>
+    unfold ValidHeadVariable at h; simp at *
+  case _ h =>
+    apply @ih C D Γ e; apply valid_insttype_subst _ _ h
+    case _ =>
+      intro n y h1
+      cases n <;> simp at *
+      case _ n => subst h1; rw [Frame.apply_compose]; simp
+    case _ =>
+      intro n h1
+      cases n <;> simp at *
+      case _ =>
+        unfold Frame.apply at h1; simp at h1
+        unfold Frame.is_stable at h1; simp at h1
+case _ Γ a A B T j1 j2 ih =>
+  cases h2
+  case _ h =>
+    unfold ValidHeadVariable at h; simp at *
+  case _ h =>
+    apply @ih C D Γ e; apply valid_insttype_subst _ _ h
+    case _ =>
+      intro n y h1
+      cases n <;> simp at *
+      case _ n => subst h1; rw [Frame.apply_compose]; simp
+    case _ =>
+      intro n h1
+      cases n <;> simp at *
+      case _ =>
+        unfold Frame.apply at h1; simp at h1
+        unfold Frame.is_stable at h1; simp at h1
+case _ B T A j ih =>
+  cases h2; case _ h =>
+    unfold ValidHeadVariable at h; simp at *
+
+theorem ctx_get_var_no_spine_eq_type:
+  ⊢ Γ ->
+  Γ.is_stable_red x ->
+  (Γ d@ x).get_type = some T ->
+  Γ ⊢ (A ~ B) : ★ ->
+  SpineType T (A ~ B) ->
+  False
+:= by
+intro h1 h2 h3 h4 h5
+have lem1 := frame_wf_by_index x h1
+simp at *; generalize fdef : Γ d@ x = f at *
+cases lem1
+all_goals (
+  unfold Frame.get_type at h3
+  unfold Frame.is_stable_red at h2; simp at *)
+case _ j => subst h3; apply spine_type_is_not_kind h5 h4 j
+case _ j => subst h3; apply spine_type_is_not_kind h5 h4 j
+case _ j1 j2 => subst h3; apply spine_type_is_not_valid_ctor rfl h5 j2
+case _ j => subst h3; apply spine_type_is_not_kind h5 h4 j
+case _ j1 j2 => subst h3; apply spine_type_is_not_valid_insttype rfl h5 j2
 
 theorem invert_eq_kind : Γ ⊢ (A ~ B) : w -> w = ★ := by
 intros eqJ; cases eqJ; simp_all;
